examples/BirthdayBook.thy
@@ -12,7 +12,7 @@ consts
 zstore BirthdayBook = 
   known :: "\<bbbP> name"
   birthday :: "name \<Zpfun> date"
-  where "known = dom birthday" "known \<subseteq> NAME" "ran(birthday) \<subseteq> DATE"
+  where "dom(birthday) = known" "known \<subseteq> NAME" "ran(birthday) \<subseteq> DATE"
 
 zoperation AddBirthday = 
   over BirthdayBook
@@ -40,15 +40,17 @@ zoperation Remind =
 lemma Remind_inv: "Remind (n, d) preserves BirthdayBook_inv"
   by zpog_full
 
-zmachine BirthdayBookSys = 
+zmachine BirthdayBookSys =
+  over BirthdayBook
   init "[known \<leadsto> {}, birthday \<leadsto> {\<mapsto>}]"
+  invariant BirthdayBook_inv
   operations AddBirthday FindBirthday Remind
 
 definition [z_defs]: "BirthdayBook_axioms = (NAME \<noteq> {} \<and> DATE \<noteq> {})"
 
-lemma BirthdayBook_deadlock_free: "BirthdayBook_axioms \<Longrightarrow> deadlock_free BirthdayBookSys"
+lemma BirthdayBook_deadlock_free: "BirthdayBook_axioms \<Longrightarrow> deadlock_free BirthdayBookSys" 
   unfolding BirthdayBookSys_def
-  by (deadlock_free "BirthdayBook_inv :: BirthdayBook \<Rightarrow> bool" invs: AddBirthday_inv FindBirthday_inv Remind_inv) 
+  by (deadlock_free invs: AddBirthday_inv FindBirthday_inv Remind_inv)
 
 def_consts NAME = "{STR ''Simon''}" 
 def_consts DATE = "{STR ''25/08/1983''}"
